work on FO.

FO.ec
@@ -1,5 +1,5 @@
 require import AllCore List Distr.
-require (*--*) ROM PKE_CPA KEM_CCA.
+require (*--*) PROM PKE_CPA KEM_CCA OW_PCVA.
 
 (* Types of public/private keys, plain-texts, ciphertexts, randomness and 
    hashes. *)
@@ -7,103 +7,72 @@ type pkey, skey, ptxt, ctxt, rand, hash.
 
 op drand : rand distr.
 axiom drand_ll : is_lossless drand.
-axiom drand_uni : is_uniform drand.
-axiom drand_full : is_full drand.
+axiom drand_funi : is_funiform drand.
 
 op dptxt : ptxt distr.
 axiom dptxt_ll : is_lossless dptxt.
-axiom dptxt_uni : is_uniform dptxt.
-axiom dptxt_full : is_full dptxt.
+axiom dptxt_funi : is_uniform dptxt.
 
-(* Key generation *)
+hint solve 0 random : drand_ll drand_funi dptxt_ll dptxt_funi.
+
+
+(**********************************************************)
+(* PKE Scheme with deterministic randomness *)
+
+  (* Key generation *)
 op kg : (pkey * skey) distr.
 
-(* Encryption, deterministic and randomized version. *)
+  (* Encryption, deterministic and randomized version. *)
 op d_enc (pk:pkey, m:ptxt, r:rand) : ctxt.
 
 op enc (pk:pkey, m:ptxt) : ctxt distr = dmap drand (d_enc pk m).
 
-op dec (pk:skey, m:ctxt) : ptxt option.
+op dec (sk:skey, c:ctxt) : ptxt option.
+
+op pk_of_sk (sk:skey) : pkey.
+
+axiom pk_of_sk_sound (sk : skey) (pk, pk' : pkey) :
+  support kg (pk, sk) => pk_of_sk sk = pk' => pk = pk'.
+
+module Scheme = {
+  proc kg () : pkey * skey = { 
+    var psk;
+    psk <$ kg;
+    return psk;
+ }
+
+  proc enc (pk:pkey, m:ptxt) : ctxt = {
+    var c;
+    c <$ enc pk m;
+    return c;
+ }
+
+  proc d_enc (pk:pkey, m:ptxt, r:rand) : ctxt = {
+    return (d_enc pk m r);
+ }
+
+  proc dec (sk:skey, c:ctxt) : ptxt option = {
+    return (dec sk c);
+ }
+}.
 
 
 (**********************************************************)
 (* Gamma-spread hypothesis necessary condition *)
 op gamma : int.
 
-module GammaCol = {
-  proc col (pk : pkey, m : ptxt, c : ctxt) : bool = {
-    var c';
-    c' <$ enc pk m;
-    return (c = c');
-  }
-}.
-
-axiom gamma_spread_coll (pk : pkey) (m : ptxt) (c : ctxt) &m:
-  Pr[GammaCol.col(pk, m, c) @ &m : res = true] <= 2%r^(-gamma).
+axiom gamma_spread_coll (pk : pkey) (m : ptxt) (c : ctxt):
+  exists (sk : skey), support kg (pk, sk) =>
+  mu1 (enc pk m) c <= 2%r^(-gamma).
 
 
 (**********************************************************)
 (* OW-PCVA Security Game *)
-
-module type OW_OraclesT = {
-  (* Plaintext checking oracle for *valid* cipher-texts *)
-  proc ptxt_check (m : ptxt, c : ctxt) : bool
-
-  (* Cipher-text validity oracle, except for the challenge cipher-text. *)
-  proc ctxt_val (c : ctxt) : bool
-}.
-
-module type Inverter (O : OW_OraclesT) = {
-  proc invert(pk : pkey, c : ctxt) : ptxt
-}.
-
-
-module OW_Oracles = {
-  var sk : skey
-  var c0 : ctxt
-
-  proc init (sk : skey, c0 : ctxt) : unit = {
-    sk <- sk;
-    c0 <- c0;
-  }
-
-  proc ptxt_check (m : ptxt, c : ctxt) : bool = {
-    var m0;
-
-    m0 <- dec sk c;    
-    return is_none m0 \/ oget m0 = m;
-  }
-
-  proc ctxt_val (c : ctxt) : bool = {
-    var m = None;
-    if (c <> c0) {
-      m <- dec sk c;
-    }
-
-    return !is_none m;
-  }
-}.
-
-module OW_Gen (I : Inverter) = {
-  proc main(): bool ={
-    var pk, sk, m, c, m';
-    var is_inv : bool;
-
-    (pk,sk) <$ kg;
-    m       <$ dptxt;
-    c       <$ enc pk m;
-    OW_Oracles.init(sk, c);
-
-    (* The adversary tries to invert C *)
-    m'      <@ I(OW_Oracles).invert(pk, c);
-
-    (* We check if m' is the invert of c using the oracle.
-       If the schema is correct here, i.e. if dec sk c = m, this corresponds
-       to checking whether m = m'. *)
-    is_inv  <@ OW_Oracles.ptxt_check (m',c);
-    return is_inv;
-  }
-}.
+clone import OW_PCVA as OW_PCVA_CPA with
+  type pkey <- pkey,
+  type skey <- skey,
+  type ptxt <- ptxt,
+  type ctxt <- ctxt.
 
 
 (**********************************************************)
@@ -114,14 +83,265 @@ clone import PKE_CPA as IND_CPA with
   type ptxt <- ptxt,
   type ctxt <- ctxt.
 
+print IND_CPA.
+
 
 (**********************************************************)
 (* KEM IND-CCA *)
-clone import KEM_CCA as IND_CCA with
+clone import KEM_CCA as KEM_INC_CCA with
   type pkey  <- pkey,
   type skey  <- skey,
   type Key   <- hash,
   type encap <- ctxt.
-  
 
-print IND_CCA.
+
+(**********************************************************)
+(* PROM *)
+type string.
+
+op s_ptxt (m : ptxt) : string.
+op s_cptxt (c : ctxt) (m : ptxt) : string.
+
+axiom s_ptxt_inj (m1 m2 : ptxt) : s_ptxt m1 = s_ptxt m2 => m1 = m2.
+axiom s_cptxt_inj (c1 c2 : ctxt) (m1 m2 : ptxt) :
+  s_cptxt c1 m1 = s_cptxt c1 m2 => m1 = m2 /\ c1 = c2.
+
+op to_rand (h : hash) : rand.
+axiom t_rand_inj (h1 h2 : hash) : to_rand h1 = to_rand h2 => h1 = h2.
+
+op dhash (m : string) : hash distr.
+axiom dhash_ll : forall m, is_lossless (dhash m).
+
+hint solve 0 random : dhash_ll.
+
+clone import PROM.GenEager as ROM with 
+  type from <- string,
+  type to <- hash,
+  op sampleto <- dhash,
+  type input <- unit,
+  type output <- bool
+  proof *. 
+  realize sampleto_ll by solve (random). 
+
+
+(**********************************************************)
+(* Correction Assumption *)
+
+module type Adv = {
+  proc a (sk : skey, pk : pkey) : ptxt
+}.
+
+module Cor (A : Adv) = {
+  proc main () = {
+    var pk, sk, r, m;
+    
+    (pk,sk) <$ kg;
+    m   <@ A.a(sk, pk);
+    r   <$ drand; 
+    return (dec sk (d_enc pk m r) <> Some m);
+  }
+}.
+
+(* Probability of error. *)
+op delt : real.
+
+(* Correction assumption. *)
+axiom corr_assum (A <: Adv) &m : Pr[Cor(A).main() @ &m: res] <= delt.
+
+
+(**********************************************************)
+(* Equivalence between the correction game and an alternative formulation, 
+  using a submit oracle. *)
+
+module type Submit = {
+  proc sub (m : ptxt) : rand
+}.
+
+module type AdvS (S : Submit) = {
+  proc a (sk : skey, pk : pkey) : unit
+}.
+
+module CorS (A : AdvS) = {
+  var m : ptxt
+  var r : rand
+  var b : bool
+  
+  module S : Submit = {
+    proc sub (m0 : ptxt) = {
+      if (!b) {
+        m <- m0;
+        b <- true;
+      }
+      return r; }}
+
+  proc main () = {
+    var pk, sk;
+    
+    m <- witness;
+    b <- false;
+    r <$ drand;
+
+    (pk,sk) <$ kg;
+    A(S).a(sk, pk);
+    return (dec sk (d_enc pk m r) <> Some m);
+  }
+}.
+
+
+(* Cor to CorS *)
+
+module B (A : Adv) (S : Submit) = {
+  proc a (sk : skey, pk : pkey) = {
+    var m;
+    m <@ A.a(sk,pk);
+    S.sub (m);    
+  }
+}.
+
+lemma Cor_to_CorS (A <: Adv {-CorS}) : 
+    equiv [CorS(B(A)).main ~ Cor(A).main: ={glob A} ==> ={res}].
+proof.
+  by proc; inline*; wp; swap {2} -2; call (_: true); auto.
+qed.
+
+
+(* CorS to Cor *)
+
+module C (A : AdvS) = {
+  var m : ptxt
+  var b : bool
+
+  module S : Submit = {
+    proc sub (m0 : ptxt) : rand = {
+      if (!b) {
+        m <- m0;
+        b <- true;
+      }
+      return witness; }}
+
+  proc a (sk : skey, pk : pkey) = {
+    m <- witness;
+    b <- false;
+    A(S).a(sk,pk);
+    return m;
+  }
+}.
+
+lemma CorS_to_Cor (A <: AdvS {-CorS, -C}) : 
+    equiv [CorS(A).main ~ Cor(C(A)).main: ={glob A} ==> ={res}].
+proof.
+ proc; inline*; swap {2} -7; wp. 
+ call (_: C.b,                  (* bad *)
+          C.b{2} = CorS.b{1} /\ C.m{2} = CorS.m{1},  (* if not bad *)
+          C.b{2} = CorS.b{1} /\ C.m{2} = CorS.m{1}). (* if bad *)
+ admit.   (* TODO: add the losslessness assumptions*)
+ proc; auto.
+ move => &2 h; proc; rcondf ^if; auto.
+ move => &1; proc; rcondf ^if; auto.
+ auto => />; smt ().
+qed.
+
+
+(**********************************************************)
+(* Transformation T : IND_CPA ==> OW_PCVA *)
+
+module T (H : ROM.RO) = {
+  proc kg () : pkey * skey = { 
+    var psk;
+    psk <$ kg;
+    return psk;
+  }
+
+  proc enc (pk:pkey, m:ptxt) : ctxt = {
+    var h, r, c;
+    h <@ H.get(s_ptxt m);
+    r <- to_rand h;
+    c <- d_enc pk m r;
+    return c;
+  }
+
+  proc dec (sk:skey, c:ctxt) : ptxt option = {
+    var m, c'; 
+
+    (* We decrypt c *)
+    m <- dec sk c;
+    (* We re-encrypt c, and check that this yields the same message. *)
+    if (!is_none m){      
+      c' <@ enc (pk_of_sk sk, oget m);
+      m <- (c = c')? m : None;
+    }
+    
+    return m;
+  }
+}.
+
+
+(**********************************************************)
+(* Game hop G0 => G1 *)
+
+module type InverterO (H : RO) (S : Scheme) (O : OraclesT) = {
+  proc invert(pk : pkey, c : ctxt) : ptxt
+}.
+
+print RO.
+
+module LH (H : RO) : RO = {
+  var log: (string * hash) list
+
+  proc init () = {
+    log <- [];
+    H.init ();
+  }
+
+  proc get(x : string) = {
+  var r;
+    
+  r    <@ H.o(x);
+  logH <- (x,r)::logH;
+  return r;
+  }
+}
+
+  module G' = {
+    proc o(x : htag) = {
+      var r;
+
+      r    <@ G.o(x);
+      logG <- (x,r)::logG;
+      return r;
+    }
+  }
+
+module Oracles0 (H : RO) = OW_PCVA_CPA.Oracles (T (H)).
+
+module Oracles1 (H : RO) = {
+  var sk : skey
+  var c0 : ctxt
+
+  proc init (sk : skey, c0 : ctxt) : unit = {
+    sk <- sk;
+    c0 <- c0;
+  }
+
+  proc ptxt_check (m : ptxt, c : ctxt) : bool = {
+    var m0, c0;
+
+    m0 <- dec sk c;
+    if (!is_none m0) {
+      c0 <@ T(H).enc (pk_of_sk sk, oget m0);
+    }
+    return is_none m0 \/ (oget m0 = m /\ c0 = c);
+  }
+
+  proc ctxt_val (c : ctxt) : bool = {
+    var m = None;
+    if (c <> c0) {
+      m <@ S.dec (sk,c);
+    }
+
+    return !is_none m;
+  }
+}.
+
+
+module Game0 (A : InverterO) (H : RO) (
